src/Init/Data/String/Decode.lean
@@ -1314,6 +1314,38 @@ public theorem isUtf8FirstByte_getElem_zero_utf8EncodeChar {c : Char} :
     ((String.utf8EncodeChar c)[0]'(by simp [c.utf8Size_pos])).IsUtf8FirstByte := by
   simp
 
+public def utf8ByteSize (c : UInt8) (_h : c.IsUtf8FirstByte) : String.Pos :=
+  if c &&& 0x80 == 0 then
+    ⟨1⟩
+  else if c &&& 0xe0 == 0xc0 then
+    ⟨2⟩
+  else if c &&& 0xf0 == 0xe0 then
+    ⟨3⟩
+  else
+    ⟨4⟩
+
+def _root_.ByteArray.utf8DecodeChar?.FirstByte.utf8ByteSize : FirstByte → String.Pos
+  | .invalid => ⟨0⟩
+  | .done => ⟨1⟩
+  | .oneMore => ⟨2⟩
+  | .twoMore => ⟨3⟩
+  | .threeMore => ⟨4⟩
+
+theorem utf8ByteSize_eq_utf8ByteSize_parseFirstByte {c : UInt8} {h : c.IsUtf8FirstByte} :
+    c.utf8ByteSize h = (parseFirstByte c).utf8ByteSize := by
+  simp [utf8ByteSize, FirstByte.utf8ByteSize, parseFirstByte]
+  split
+  · simp
+  · split
+    · simp
+    · split
+      · simp
+      · obtain (h|h|h|h) := h
+        · contradiction
+        · contradiction
+        · contradiction
+        · simp [h]
+
 end UInt8
 
 public theorem ByteArray.isUtf8FirstByte_getElem_zero_utf8EncodeChar_append {c : Char} {b : ByteArray} :
@@ -1329,3 +1361,20 @@ public theorem ByteArray.isUtf8FirstByte_of_isSome_utf8DecodeChar? {b : ByteArra
   obtain ⟨c, hc⟩ := Option.isSome_iff_exists.1 h
   conv => congr; congr; rw [eq_of_utf8DecodeChar?_eq_some hc]
   exact isUtf8FirstByte_getElem_zero_utf8EncodeChar_append
+
+theorem Char.byteIdx_utf8ByteSize_getElem_utf8EncodeChar {c : Char} :
+    (((String.utf8EncodeChar c)[0]'(by simp [c.utf8Size_pos])).utf8ByteSize
+      UInt8.isUtf8FirstByte_getElem_zero_utf8EncodeChar).byteIdx = c.utf8Size := by
+  rw [UInt8.utf8ByteSize_eq_utf8ByteSize_parseFirstByte]
+  obtain (hc|hc|hc|hc) := c.utf8Size_eq
+  · rw [parseFirstByte_utf8EncodeChar_eq_done hc, FirstByte.utf8ByteSize, hc]
+  · rw [parseFirstByte_utf8EncodeChar_eq_oneMore hc, FirstByte.utf8ByteSize, hc]
+  · rw [parseFirstByte_utf8EncodeChar_eq_twoMore hc, FirstByte.utf8ByteSize, hc]
+  · rw [parseFirstByte_utf8EncodeChar_eq_threeMore hc, FirstByte.utf8ByteSize, hc]
+
+public theorem ByteArray.utf8Size_utf8DecodeChar {b : ByteArray} {i} {h} :
+    (utf8DecodeChar b i h).utf8Size =
+      ((b[i]'(lt_size_of_isSome_utf8DecodeChar? h)).utf8ByteSize (isUtf8FirstByte_of_isSome_utf8DecodeChar? h)).byteIdx := by
+  rw [← Char.byteIdx_utf8ByteSize_getElem_utf8EncodeChar]
+  simp only [List.getElem_eq_getElem_toByteArray, utf8EncodeChar_utf8DecodeChar]
+  simp [ByteArray.getElem_extract]
